
\documentclass[12pt,a4paper]{book}

\usepackage{eqcode}

\begin{document}

\begin{eqcode}{mod}{v, d}{\type{Z},\type{Z}}{\type{Z}}
	res = {(v+d) \mod d } \lend
	\return {res}
\end{eqcode}

\begin{eqcode}{simps}{f, h}{\type{R}^1,\type{R}^1}{\type{R}^1}
	r \in \type{R}^2_{100, 80} \lend
	n = \call{shape}{f}_0 \lend
	undef = \genAr \limits^{\call{drop}{[1], \call{shape}{f}}} 0.0 \lend
	r_i\  |\  i \in [0,n-1] =
	\begin{cases}
		\dfrac{11.0 \cdot f_0+14.0 \cdot f_1-f_2}{24.0} & i=0 \lend	
		\dfrac{f_{i-1}+4.0 \cdot f_i+f_{i+1}}{3.0} & 1 \leq i \leq n-2 \lend
		undef & \otherwise
	\end{cases}
	\lend	
	rs = r_2	\lend
	r_2 = r_1	\lend
	r_1 = r_0	\lend
	r_0 = undef \lend
    r^{[i]}_i = r^{[i-2]}_{i-2} + rs^{[i-1]} \lend
	rs^{[i]} = r^{[i-1]}_{i-1} \lend
	\filter{r^{[i]}\  |\  i=n-1} \lend
	\return {r \cdot h}
\end{eqcode}

\begin{eqcode}{N}{u,dx,dy}{\type{R}^2,\type{R}^1,\type{R}^1}{\type{R}^2}
	undef = \genAr \limits^{\call{drop}{[1], \call{shape}{u}}} 0.0 \lend
	z_{i,j}\  |\  [i,j : 0 \leq i \leq s_0 \land  0 \leq j \leq s_1]
 =  
	\begin{cases}
		\dfrac{u_{i,j+1} - 2.0 \cdot u_{i,j} + u_{i,s_1-1}}{dy \cdot dy} 
			& [i,j: 0 \leq i \leq s_0 \land  0 \leq j \leq 1] \lend
		\dfrac{u_{i,j+1} - 2.0 \cdot u_{i,j} + u_{i,j-1}}{dy \cdot dy} 
			& [i,j : 0 \leq i \leq s_0-1 \land  0 \leq j \leq s_0-1] \lend
		\dfrac{u_{i,0}-2.0 \cdot u{i,j} + u{i,j-1}}{dy \cdot dy}
			& [i,j : 0 \leq i \leq s_0 \land  s_1-1 \leq j \leq s_1] \lend
		0.0 
			& \otherwise	\end{cases} \lend
	du_i\  |\  i \in [0,\call{take}{[1],s}] = 
	\begin{cases}
		\dfrac{u_{i+1}-u_{i-1}}{2.0 \cdot dx} & 1 \leq i \leq s_0-2 \lend
		undef & \text{otherwise}
	\end{cases}
	\lend
	du_0 = \dfrac{u_1-u_0}{ dx} \lend
	du_{s_0-1} = \dfrac{u_{s_0-1}-u_{s_0}-2}{dx} \lend
	\return {3.0 \cdot \call{simps}{z,dx}-6.0 \cdot u \cdot du}
\end{eqcode}

\begin{eqcode}{L}{u, dx}{\type{R}^1,\type{R}^1}{\type{R}^1}
	undef = \genAr \limits^{\call{drop}{[1] ,\call{shape}{u}}} 0.0 \lend
	s = \call{shape}{u}_0 \lend
	z_i\  |\  i \in [0, \call{take}{[1], \call{shape}{u}}] =  
	\begin{cases}
		- \dfrac{u_{i+2}-2.0 \cdot u_{i+1} + 2.0 
				\cdot u_{i-1} - u_{i-2}}{ 2.0 \cdot dx \cdot dx \cdot dx} 
			& 2 \leq i \leq s-3 \lend
		undef 
			& \otherwise \lend
	\end{cases} \lend
	z_0 = - \dfrac{u_0 -2.0 \cdot u_1 + u_2}{dx \cdot dx \cdot dx}
\lend
	z_1 = - \dfrac{-u_0 + 3.0 \cdot u_1 - 3.0 \cdot u_2 + u_3}{ dx \cdot dx
    \cdot dx} \lend
	z_{s-2} = - \dfrac{-u_{s-4} + 3.0 \cdot u_{s-3} -3.0 \cdot u_{s-2} +
    u_{s-1}}{ dx \cdot dx \cdot dx} \lend
	z_{s-1} = \dfrac{u_{s-3} - 2.0 \cdot u_{s-2} + u_{s-1}}{ dx \cdot dx \cdot
    dx} \lend
	\return {x}
\end{eqcode}

\begin{eqcode}{prepent}{a,b,c,d,e}{\type{R}^1, \type{R}^1, \type{R}^1, \type{R}^1, \type{R}^1}{\type{R}^1, \type{R}^1, \type{R}^1, \type{R}^1}
	n = \call{shape}{a}_0 \lend
	undef = \genAr \limits^{\call{drop}{[1], \call{shape}{a}}} 0.0 \lend
	p = q = bet = den = \genAr \limits^{n} undef \lend
	bet_0 = \dfrac{1.0}{c_0} \lend
	p_0 = -d_0 \cdot bet_0 \lend
	q_0 = -e_0 \cdot bet_0 \lend
	bet_1 = - \dfrac{1.0}{c_1+b_1 \cdot p_0} \lend
	p_1 = (d_1+b_1 \cdot q_0) \cdot bet_1 \lend
	q_1 = e_1 \cdot bet_1 \lend
	den_1 = b_1 \lend
    p^{[0]}_0 = p_0, p^{[1]}_1 = p_1, q^{[0]}_0 = q_0, q^{[1]}_1 = q_1 \lend
    bet^{[i]}_{i} = b_i + a_i \cdot p^{[i-2]}_{i-2} \lend
	den^{[i]}_i = -\dfrac{1.0}{c_i +a_i \cdot q^{[i-2]}_{i-2} + bet^{[i]}_i
    \cdot p^{[i-1}]_{i-1}} \lend
	p^{[i]}_i = (d_i + bet^{[i]}_i \cdot q^{[i-1]})_{i-1} \cdot den^{[i]}_i \lend
	q^{[i]}_i = e_i \cdot den^{[i]}_i \lend
	\filter{p^{[i]}, q^{[i]}, bet^{[i]}, den^{[i]}\  |\  i=n-1} \lend
	\return {p,q,bet,den} \lend
\end{eqcode}

\begin{eqcode}{pent}{p,q,bet,den,a,u}{\type{R}^1_{100}, \type{R}^1_{100}, \type{R}^1_{100}, \type{R}^1_{100}, \type{R}^1_{100}, \type{R}^2_{100,80}}{\type{R}^2}
	n = \call{shape}{a}_0 \lend
	n_0 = u_0 \cdot bet_0 \lend
	u_1 = (den_1 \cdot u_0 - u_1) \cdot bet_1 \lend
    u^{[0]}_1 = u_1 \lend
    u^{[1]}_2 = u_2 \lend
    u^{[2]}_3 = u_3 \lend
	u^{[i]}_i = (a_i \cdot u^{[i-3]}_{i-2} + bet_i \cdot u^{[i-2]}_{i-1}-u^{[i-1]}_i) \cdot den_i \lend
	\filter{u^{[i]}\  |\  i=n-1} \lend
    u^{[0]} = u \lend
	u_{n-2} = u_{n-2} + p_{n-2} \cdot u_{n-1} \lend
	u^{[i]}_{n-3-i} = u^{[i-1]}_{n-3-i} + p_i \cdot u^{[i-1]}_{n-4-i} + q_i \cdot u^{[i-1]}_{n-5-i} \lend
	\filter{u^{[i]}\  |\  i=n-3} \lend
	\return {u} \lend
\end{eqcode}

\begin{eqcode}{soliton}{x,y}{\type{R}^1, \type{R}^1}{\type{R}^1}
	k = frac(\sqrt{6.0}, 4.0) \lend
	num = -4.0 \cdot x \cdot x + 15.0 \cdot k \cdot k \cdot y \cdot y + \dfrac{1.0}{k \cdot k} \lend
	denom = 4.0 \cdot x \cdot x + 16.0 \cdot k \cdot k \cdot y \cdot y +
    \dfrac{1.0}{k \cdot k} \lend
	\return {\dfrac{16.0 \cdot num}{denom \cdot denom}} \lend
\end{eqcode}

\begin{eqcode}{main}{a,b,c,d,e,p,q,bet,den,u,f}{\type{R}^2_{100,3}, \type{R}^2_{100,3}, \type{R}^2_{100,3}, \type{R}^2_{100,3},  \type{R}^2_{100,3},  \type{R}^2_{100,3}, \type{R}^2_{100,3}, \type{R}^2_{100,3}, \type{R}^2_{100,3}, \type{R}^2{100,80}, \type{R}^2_{100,80}}{\type{Z}}
	niter = \call{FibreScanIntArray}{} \lend
	out = 0 \lend
	undef = 0.0 \lend
	dx = 0.1 \lend
	dy = 0.1 \lend
	dt = 0.0002 \lend
	n = 100 \lend
	m = 80 \lend
	ymax = frac(\call{tod}{n} \cdot dx, 2.0) \lend
	xmin = -xmax \lend
	ymax = frac(\call{tod}{m} \cdot dy, 2.0) \lend
	ymin = -ymax \lend
	alpha = [\dfrac{8.0}{15.0}, \dfrac{2.0}{15.0}, \dfrac{1.0}{3.0}] \cdot dt \lend
	gamma = [\dfrac{8.0}{15.0}, \dfrac{5.0}{5.0}, \dfrac{3.0}{4.0}] \cdot dt \lend
	rho = [\dfrac{-17.0}{60.0}, \dfrac{-5.0}{12.0}] \cdot dt \lend
	eps = \dfrac{alpha}{4.0 \cdot dx \cdot dx \cdot dx} \lend
	mins = [\call{tof}{xmin}, \call{tof}{ymin}, -2f] \lend
	maxs = [\call{tof}{xmax}, \call{tof}{ymax}, 8f] \lend
	steps = [5f, 4f, 2f] \lend
	u_{i,j}\  |\  [i, j : 0 \leq i \leq n \land  0 \leq i \leq m] =
 	\begin{cases}
		\call{soliton}{xmin + dx \cdot \call{tod}{i}},\  ymin+dy \cdot \call{tod}{j} 
			& [i, j : 0 \leq i \leq n \land 0 \leq j \leq m] \lend
		undef 
			& \otherwise
	\end{cases}
	\lend
	a = \genAr \limits^{n} -eps \lend
	a_0 = [0.0, 0.0, 0.0] \lend
	a_1 = [0.0, 0.0, 0.0] \lend
	a_{n-2} = 2.0 \cdot a_{n-3} \lend
	a_{n-1} = a_{n-2} \lend
	b = \genAr \limits^{n} (2.0 \cdot eps) \lend
	b_0 = [0.0, 0.0, 0.0] \lend
	b_1 = -b_2 \lend
	b_{n-2} = 3.0 \cdot b_{n-3} \lend
	b_{n-1} = 2.0 \cdot b_{n-3} \lend
	c = \genAr \limits^{n \times 3} 1.0 \lend
	c_0 = c_0 + 2.0 \cdot eps \lend
	c_1 = c_1 + 6.0 \cdot eps \lend
	c_{n-2} = c_{n-2} - 6.0 \cdot eps \lend
	c_{n-1} = c_{n-1} -2.0 \cdot eps \lend
	d = \genAr \limits^{n} (-2.0 \cdot eps) \lend
	d_0 = 2.0 \cdot d_2 \lend
	d_1 = 3.0 \cdot d_2 \lend
	d_{n-2} = -d{n-3} \lend
	d_{n-1} = [0.0, 0.0, 0.0] \lend
	e = \genAr \limits^{n} eps \lend
	e_0 = 2.0 \cdot e_2 \lend
	e_1 = e_0 \lend
	e_{n-2} = [0.0, 0.0, 0.0] \lend
	e_{n-1} = [0.0, 0.0, 0.0] \lend
	p, q, bet, den = \call{prepent}{a,b,c,d,e} \lend
	\left.\begin{aligned}
		Nubase = \call{N}{u, dx, dy} \lend
		f = u + gamma_0 \cdot Nubase + alpha_0 \cdot 0.5 \cdot \call{L}{u, dx} \lend
		u = \call{pent}{p_{.,0},q_{.,0},bet{.,0},den{.,0},a{.,0},f} \lend
		Nunext = \call{N}{u, dx, dy} \lend
		f = u + gamma_1 \cdot Nunext + rho_0 \cdot Nubase + alpha_1 \cdot 0.5 \cdot \call{u, dx} \lend
		u = \call{pent}{p_{.,1}, q{.,1}, bet{.,1},den{.,1},a{.,1},f} \lend
		f = u + gamma_2 \cdot \call{N}{u, dx, dy} + rho_i \cdot Nunext + alpha_2 \cdot 0.5 \cdot \call{L}{u,dx} \lend
		u = \call{pent}{p_{.,2},q_{.,2},bet{.,2},den{.,2},a{.,2},f} \lend

		\end{aligned}
	\right\} 
	\  1 \leq iter \leq niter-1 \lend
	\text{print} \call{maxval}{\call{abs}{u}} \lend
	\return (0) \lend
\end{eqcode}
\end{document}
